veric/semax_loop.v
@@ -1,3 +1,4 @@
+Load loadpath. 
 Require Import veric.base.
 Require Import msl.normalize.
 Require Import veric.Address.
